Code/Prelude/Wellfounded.v
@@ -1,17 +1,17 @@
 (** * Well-founded types *)
 
 (** To formulate well-foundedness constructively, we make use of inductive subsets. *)
-Inductive isWf {X : Type} (R : X -> X -> Prop) (x : X) : Prop :=
+Inductive isWf {X : Type} (R : X -> X -> Type) (x : X) : Prop :=
 | acc : (forall (y : X), R x y -> isWf R y) -> isWf R x.
 
-Definition Wf {X : Type} (R : X -> X -> Prop)
+Definition Wf {X : Type} (R : X -> X -> Type)
   := forall (x : X), isWf R x.
 
 (** Well-founded types are closed under inverse images *)
 Lemma fiber_is_Wf_help
       {X Y : Type}
-      {RX : X -> X -> Prop}
-      {RY : Y -> Y -> Prop}
+      {RX : X -> X -> Type}
+      {RY : Y -> Y -> Type}
       {f : X -> Y}
       (Hf : forall (x1 x2 : X), RX x1 x2 -> RY (f x1) (f x2))
       (y : Y)
@@ -31,8 +31,8 @@ Qed.
 
 Proposition fiber_is_Wf
             {X Y : Type}
-            {RX : X -> X -> Prop}
-            {RY : Y -> Y -> Prop}
+            {RX : X -> X -> Type}
+            {RY : Y -> Y -> Type}
             (HY : Wf RY)
             (f : X -> Y)
             (Hf : forall (x1 x2 : X), RX x1 x2 -> RY (f x1) (f x2))
@@ -46,7 +46,7 @@ Qed.
 
 (** If a type is well-founded, then there are no infinite decreasing chains in it *)
 
-Record infinite_chain {X : Type} (R : X -> X -> Prop) :=
+Record infinite_chain {X : Type} (R : X -> X -> Type) :=
   {
     seq :> nat -> X ;
     decr : forall (n : nat), R (seq n) (seq (S n))
@@ -56,7 +56,7 @@ Arguments decr {_} {_} _ _.
 
 Definition shift
            {X : Type}
-           {R : X -> X -> Prop}
+           {R : X -> X -> Type}
            (f : infinite_chain R)
   : infinite_chain R
   := {| seq n := f (S n) ;
@@ -64,7 +64,7 @@ Definition shift
 
 Definition no_infinite_chain_help
            {X : Type}
-           (R : X -> X -> Prop)
+           (R : X -> X -> Type)
            (HX : Wf R)
   : forall (x : X)
            (f : infinite_chain R)
@@ -85,7 +85,7 @@ Qed.
 
 Definition no_infinite_chain
            {X : Type}
-           (R : X -> X -> Prop)
+           (R : X -> X -> Type)
            (HX : Wf R)
   : infinite_chain R -> False.
 Proof.
