Code/Syntax/Signature/Terms.v
@@ -1,3 +1,4 @@
+Require Import Prelude.Basics.
 Require Import Syntax.Signature.Types.
 Require Import Syntax.Signature.Contexts.
 
@@ -21,3 +22,305 @@ Arguments App {_} {_} {_} {_} {_} {_} _ _.
 
 Notation "'λ' x" := (Lam x) (at level 10) : signature.
 Notation "f · x" := (App f x) (at level 20, left associativity) : signature.
+
+(** * Decidable alpha equality of terms *)
+Definition is_BaseTm
+           {B : Type}
+           {F : Type}
+           {ar : F -> ty B}
+           {C : con B}
+           {A : ty B}
+           (t : tm ar C A)
+  : Prop
+  := match t with
+     | BaseTm _ => True
+     | _ => False
+     end.
+
+Definition transport_BaseTm
+           {B : Type}
+           {F : Type}
+           {ar : F -> ty B}
+           {C : con B}
+           {A1 A2 : ty B}
+           (t : tm ar C A1)
+           (p : A1 = A2)
+           (Ht : is_BaseTm t)
+  : is_BaseTm (transport (tm ar C) p t).
+Proof.
+  subst.
+  simpl.
+  exact Ht.
+Qed.
+
+Definition is_BaseTm_at
+           {B : Type}
+           {F : Type}
+           {ar : F -> ty B}
+           {C : con B}
+           {A : ty B}
+           (f : F)
+           (t : tm ar C A)
+  : Prop
+  := match t with
+     | BaseTm f' => f = f'
+     | _ => False
+     end.
+
+Definition transport_BaseTm_at
+           {B : Type}
+           {F : Type}
+           {ar : F -> ty B}
+           {C : con B}
+           {A1 A2 : ty B}
+           (f : F)
+           (t : tm ar C A1)
+           (p : A1 = A2)
+           (Ht : is_BaseTm_at f t)
+  : is_BaseTm_at f (transport (tm ar C) p t).
+Proof.
+  subst.
+  simpl.
+  exact Ht.
+Qed.
+
+Definition is_Lambda
+           {B : Type}
+           {F : Type}
+           {ar : F -> ty B}
+           {C : con B}
+           {A : ty B}
+           (t : tm ar C A)
+  : Prop
+  := match t with
+     | λ _ => True
+     | _ => False
+     end.
+
+Definition transport_Lambda
+           {B : Type}
+           {F : Type}
+           {ar : F -> ty B}
+           {C : con B}
+           {A1 A2 : ty B}
+           (t : tm ar C A1)
+           (p : A1 = A2)
+           (Ht : is_Lambda t)
+  : is_Lambda (transport (tm ar C) p t).
+Proof.
+  subst.
+  simpl.
+  exact Ht.
+Qed.
+
+Definition tm_dec_eq_help
+           {B : Type}
+           {F : Type}
+           `{decEq B}
+           `{decEq F}
+           {ar : F -> ty B}
+           {C : con B}
+           {A1 A2 : ty B}
+           (t1 : tm ar C A1)
+           (t2 : tm ar C A2)
+           (p : A1 = A2)
+  : dec (transport (tm ar C) p t1 = t2).
+Proof.
+  revert p.
+  revert t2.
+  revert A2.
+  induction t1 ; intros ? t2 p.
+  - (* t1 is a base term *)
+    destruct t2.
+    + (* t2 is a base term *)
+      destruct (dec_eq f f0).
+      * refine (Yes _).
+        abstract
+          (subst ;
+           rewrite (hedberg p eq_refl) ;
+           reflexivity).
+      * refine (No _).
+        abstract
+          (intro q ;
+           pose (transport
+                   (is_BaseTm_at f)
+                   q
+                   (transport_BaseTm_at f (BaseTm f) p eq_refl))
+             as r ;
+           cbn in r ;
+           contradiction).
+    + (* t2 is a variable *)
+      refine (No _).
+      abstract
+        (subst ;
+         discriminate).
+    + (* t2 is a lambda abstraction *)
+      refine (No _).
+      abstract
+        (intro q ; 
+         exact (transport is_BaseTm q (transport_BaseTm (BaseTm f) p I))).
+    + (* t2 is an application *)
+      refine (No _).
+      abstract
+        (subst ;
+         discriminate).
+  - (* t1 is a variable *)
+    destruct t2.
+    + (* t2 is a base term *)
+      refine (No _).
+      abstract
+        (subst ;
+         discriminate).
+    + (* t2 is a variable *)
+      destruct (dec_eq (transport (var C) p v) v0).
+      * refine (Yes _).
+        abstract
+          (subst ;
+           reflexivity).
+      * refine (No _).
+        abstract
+          (intro q ;
+           subst ;
+           simpl in * ;
+           inversion q ;
+           pose (path_in_sigma_uip _ H2) ;
+           contradiction).
+    + (* t2 is a lambda abstraction *)
+      refine (No _).
+      abstract
+        (subst ;
+         discriminate).
+    + (* t2 is an application *)
+      refine (No _).
+      abstract
+        (subst ;
+         discriminate).
+  - (* t1 is a lambda abstraction *)
+    destruct t2.
+    + (* t2 is a base term *)
+      refine (No _).
+      abstract
+        (intro q ;
+         refine ((transport is_Lambda q (transport_Lambda (λ t1) p I)))).
+    + (* t2 is a variable *)
+      refine (No _).
+      abstract
+        (subst ;
+         discriminate).
+    + (* t2 is a lambda abstraction *)
+      inversion p.
+      induction H2.
+      destruct (IHt1 _ t2 H3).
+      * refine (Yes _).
+        abstract
+          (subst ; simpl ;
+           rewrite (hedberg p eq_refl) ;
+           reflexivity).
+      * refine (No _).
+        abstract
+          (intro q ;
+           subst ;
+           simpl in * ;
+           rewrite (hedberg p eq_refl) in q ;
+           simpl in q ;
+           inversion q; 
+           pose (path_in_sigma_uip _ H2) as e ;
+           pose (path_in_sigma_uip _ e) ;
+           contradiction).
+    + (* t2 is an application *)
+      refine (No _).
+      abstract
+        (subst ;
+         discriminate).
+  - (* t1 is an application *)
+    destruct t2.
+    + (* t2 is a base term *)
+      refine (No _).
+      abstract
+        (subst ;
+         simpl ;
+         discriminate).
+    + (* t2 is a variable *)
+      refine (No _).
+      abstract
+        (subst ;
+         discriminate).
+    + (* t2 is a lambda abstraction *)
+      refine (No _).
+      abstract
+        (subst ;
+         discriminate).
+    + (* t2 is an application *)
+      destruct (dec_eq A1 A0).
+      * assert (pq : (A1 ⟶ A2) = (A0 ⟶ A3)).
+        {
+          subst.
+          reflexivity.
+        }
+        destruct (IHt1_1 _ t2_1 pq) as [q | q], (IHt1_2 _ t2_2 e) as [n | n].
+        ** refine (Yes _).
+           abstract
+             (subst ;
+              rewrite (hedberg pq eq_refl) ;
+              reflexivity).
+        ** refine (No _).
+           abstract
+             (intro r ;
+              subst ;
+              simpl in * ;
+              rewrite (hedberg pq eq_refl) in r ;
+              simpl in r ;
+              inversion r ;
+              pose (path_in_sigma_uip _ H2) as e ;
+              contradiction).
+        ** refine (No _).
+           abstract
+             (intro r ;
+              subst ;
+              rewrite (hedberg pq eq_refl) in q ;
+              simpl in * ;
+              inversion r ;
+              pose (path_in_sigma_uip _ H2) as e ;
+              pose (path_in_sigma_uip _ e) ;
+              contradiction).
+        ** refine (No _).
+           abstract
+             (intro r ;
+              subst ;
+              rewrite (hedberg pq eq_refl) in q ;
+              simpl in * ;
+              inversion r ;
+              pose (path_in_sigma_uip _ H3) ;
+              contradiction).
+      * refine (No _).
+        abstract
+          (intro q ;
+           subst ;
+           simpl in * ;
+           inversion q ;
+           contradiction).
+Defined.
+
+Definition tm_dec_eq
+           {B : Type}
+           {F : Type}
+           `{decEq B}
+           `{decEq F}
+           {ar : F -> ty B}
+           {C : con B}
+           {A : ty B}
+           (t1 : tm ar C A)
+           (t2 : tm ar C A)
+  : dec (t1 = t2)
+  := tm_dec_eq_help t1 t2 eq_refl.
+
+Global Instance tm_decEq
+       {B : Type}
+       {F : Type}
+       `{decEq B}
+       `{decEq F}
+       (ar : F -> ty B)
+       (C : con B)
+       (A : ty B)
+  : decEq (tm ar C A)
+  := {| dec_eq := tm_dec_eq |}.
