Code/Syntax/StrongNormalization/BetaReductionSN.v
@@ -1,0 +1,895 @@
+Require Import Prelude.Basics.
+Require Import Prelude.Wellfounded.
+Require Import Syntax.Signature.
+Require Import Syntax.Signature.SubstitutionLemmas.
+Require Import Syntax.StrongNormalization.SN.
+Require Import Coq.Program.Equality.
+
+(** * Strongly normalizing terms *)
+Definition term_isSN
+           {B : Type}
+           {F : Type}
+           {ar : F -> ty B}
+           {C : con B}
+           {A : ty B}
+           (t : tm ar C A)
+  : Prop
+  := isWf (fun (t1 t2 : tm ar C _) => betaRed t1 t2) t.
+
+(** Base terms and variables are strongly normalizing *)
+Lemma is_BaseTm_transport
+      {B : Type}
+      {F : Type}
+      {ar : F -> ty B}
+      {C : con B}
+      {A1 A2 : ty B}
+      (p : A1 = A2)
+      (t : tm ar C A1)
+  : is_BaseTm (transport _ p t) -> is_BaseTm t.
+Proof.
+  subst.
+  exact (fun x => x).
+Qed.
+
+Lemma baseTm_is_nf_help
+      {B : Type}
+      {F : Type}
+      {ar : F -> ty B}
+      {C : con B}
+      {A : ty B}
+      (t1 t2 : tm ar C A)
+      (f : F)
+      (p1 : ar f = A)
+      (p2 : transport (tm ar C) p1 (BaseTm f) = t1)
+  : betaRed t1 t2 -> False.
+Proof.
+  intro q.
+  revert p2.
+  revert p1.
+  revert f.
+  induction q ; intros f' p1 p2.
+  - apply (IHq1 f' p1 p2).
+  - subst.
+    discriminate p2.
+  - subst.
+    discriminate p2.
+  - apply (is_BaseTm_transport (eq_sym p1) (λ f1)).
+    rewrite <- p2.
+    rewrite transport_sym_p.
+    simpl.
+    auto.
+  - subst.
+    cbn in *.
+    discriminate p2.
+Qed.
+
+Lemma baseTm_is_nf
+      {B : Type}
+      {F : Type}
+      {ar : F -> ty B}
+      {C : con B}
+      (f : F)
+      (t : tm ar C (ar f))
+  : betaRed (BaseTm f) t -> False.
+Proof.
+  exact (baseTm_is_nf_help (BaseTm f) t f eq_refl eq_refl).
+Qed.
+
+Proposition baseTm_is_SN
+            {B : Type}
+            {F : Type}
+            {ar : F -> ty B}
+            {C : con B}
+            (f : F)
+  : @term_isSN _ _ ar C _ (BaseTm f).
+Proof.
+  unfold term_isSN.
+  apply acc.
+  intros ? p.
+  contradiction (baseTm_is_nf f _ p).
+Qed.
+
+Lemma var_is_nf
+      {B : Type}
+      {F : Type}
+      {ar : F -> ty B}
+      {C : con B}
+      {A : ty B}
+      (v : var C A)
+      (t : tm ar C A)
+  : betaRed (TmVar v) t -> False.
+Proof.
+  intro p.
+  dependent induction p.
+  apply (IHp1 v).
+  reflexivity.
+Qed.
+
+Proposition var_is_SN
+            {B : Type}
+            {F : Type}
+            {ar : F -> ty B}
+            {C : con B}
+            {A : ty B}
+            (v : var C A)
+  : @term_isSN _ _ ar _ _ (TmVar v).
+Proof.
+  apply acc.
+  intros ? q.
+  contradiction (var_is_nf v _ q).
+Qed.
+
+(** Closed under weakening *)
+Definition betaRed_wkTm
+           {B : Type}
+           {F : Type}
+           {ar : F -> ty B}
+           {C1 C2 : con B}
+           {w : wk C1 C2}
+           {A : ty B}
+           {t2 : tm ar C2 A}
+           {t1 : tm ar C1 A}
+           (r : betaRed (wkTm t2 w) t1)
+  : { t' : tm ar C2 A | t1 = wkTm t' w }.
+Proof.
+  (*
+  revert r.
+  revert t1.
+  revert w.
+  revert C1.
+  induction t2 ; simpl in * ; intros C1 w t1 r.
+  - contradiction (@baseTm_is_nf B F ar C1 f _ r).
+  - admit.
+  - admit.
+  - specialize (IHt2_1 _ w).
+    specialize (IHt2_2 _ w).
+
+      
+  dependent induction r.
+  - specialize (IHr1 _ w t2 eq_refl).
+    destruct IHr1 as [ t1' Ht1'].
+    exact (IHr2 _ w t1' Ht1').
+  - specialize (IHr _ w).
+    admit.
+  - specialize (IHr _ w).
+    admit.
+  - admit.
+  - admit.
+   *)
+Admitted.
+
+(*
+Proposition betaRed_wkTm_from_red
+            {B : Type}
+            {F : Type}
+            {ar : F -> ty B}
+            {C1 C2 : con B}
+            (w : wk C1 C2)
+            {A : ty B}
+            {t1 : tm ar C1 A}
+            {t2 : tm ar C2 A}
+            (r : betaRed (wkTm t2 w) t1)
+  : betaRed t2 (betaRed_wkTm r).
+Proof.
+Admitted.
+
+Proposition betaRed_wkTm_to_red
+            {B : Type}
+            {F : Type}
+            {ar : F -> ty B}
+            {C1 C2 : con B}
+            (w : wk C1 C2)
+            {A : ty B}
+            {t1 : tm ar C1 A}
+            {t2 : tm ar C2 A}
+            (r : betaRed (wkTm t2 w) t1)
+  : betaRed (wkTm (betaRed_wkTm r) w) t1.
+Proof.
+Admitted.
+ *)
+
+Proposition wkTm_isSN
+            {B : Type}
+            {F : Type}
+            {ar : F -> ty B}
+            {C1 C2 : con B}
+            (w : wk C1 C2)
+            {A : ty B}
+            (t : tm ar C2 A)
+            (p : term_isSN t)
+  : term_isSN (wkTm t w).
+Proof.
+  induction p as [t Ht IHt].
+  apply acc.
+  intros y r.
+  (*
+  pose (t' := betaRed_wkTm r).
+  destruct t' as [t' Ht'].
+  subst.
+  apply IHt.
+   *)
+Admitted.
+
+(** * Logical relations *)
+
+(** On terms *)
+Fixpoint logical_SN
+         {B : Type}
+         {F : Type}
+         {ar : F -> ty B}
+         {C : con B}
+         {A : ty B}
+  : tm ar C A -> Prop
+  := match A with
+     | Base b => term_isSN
+     | A1 ⟶ A2 =>
+       fun f =>
+         forall (C2 : con B)
+                (w : wk C2 C)
+                (t : tm ar C2 A1),
+           logical_SN t -> logical_SN (wkTm f w · t)
+     end.
+
+(** Preservation under weakening *)
+Proposition wk_logical_SN
+            {B : Type}
+            {F : Type}
+            {ar : F -> ty B}
+            {C1 C2 : con B}
+            (w : wk C1 C2)
+            {A : ty B}
+            (t : tm ar C2 A)
+            (Ht : logical_SN t)
+  : logical_SN (wkTm t w).
+Proof.
+  destruct A.
+  - apply wkTm_isSN.
+    exact Ht.
+  - intros C w' t' Ht'.
+    rewrite wkTm_comp.
+    exact (Ht _ (compWk w w') t' Ht').
+Qed.
+
+(** On substitutions *)
+Definition logical_SN_sub
+           {B : Type}
+           {F : Type}
+           {ar : F -> ty B}
+           {C1 C2 : con B}
+           (s : sub ar C1 C2)
+  : Prop
+  := forall (A : ty B)
+            (v : var C2 A),
+    logical_SN (subVar v s).
+
+(** Some constructions for logical substitutions *)
+Proposition ToEmpty_logical_SN
+            {B : Type}
+            {F : Type}
+            {ar : F -> ty B}
+            (C : con B)
+  : logical_SN_sub (@ToEmpty _ _ ar C).
+Proof.
+  intros A v.
+  inversion v.
+Qed.
+
+Proposition Extend_logical_SN
+            {B : Type}
+            {F : Type}
+            {ar : F -> ty B}
+            {C1 C2 : con B}
+            {s : sub ar C1 C2}
+            {A : ty B}
+            (t : tm ar C1 A)
+            (p : logical_SN_sub s)
+            (q : logical_SN t)
+  : logical_SN_sub (s & t).
+Proof.
+  intros A' v.
+  dependent induction v ; simpl ; cbn.
+  - exact q.
+  - apply p.
+Qed.
+
+Proposition Extend_logical_SN_pr1
+            {B : Type}
+            {F : Type}
+            {ar : F -> ty B}
+            {C1 C2 : con B}
+            {s : sub ar C1 C2}
+            {A : ty B}
+            (t : tm ar C1 A)
+            (p : logical_SN_sub (s & t))
+  : logical_SN_sub s.
+Proof.
+  intros A' v.
+  assert (subVar v s
+          =
+          subTm (TmVar (wkVar v (dropId C2 _))) (s & t)).
+  {
+    rewrite wkVar_is_subVar.
+    symmetry.
+    etransitivity.
+    {
+      apply (subTm_comp (TmVar v)).
+    }
+    simpl.
+    f_equal.
+    rewrite dropSub_is_compSubWk.
+    rewrite <- compSub_compWkSub.
+    simpl ; cbn.
+    rewrite wkToSub_id.
+    rewrite Sub_id_left.
+    rewrite compWkSub_id.
+    reflexivity.
+  }
+  rewrite H.
+  apply p.
+Qed.
+
+Proposition Extend_logical_SN_pr2
+            {B : Type}
+            {F : Type}
+            {ar : F -> ty B}
+            {C1 C2 : con B}
+            {s : sub ar C1 C2}
+            {A : ty B}
+            (t : tm ar C1 A)
+            (p : logical_SN_sub (s & t))
+  : logical_SN t.
+Proof.
+  exact (p A Vz).
+Qed.
+
+(** * Neutral terms *)
+Inductive is_neutral
+          {B : Type}
+          {F : Type}
+          {ar : F -> ty B}
+          {C : con B}
+  : forall {A : ty B}, tm ar C A -> Prop
+  :=
+| BaseTm_is_neutral : forall (f : F), is_neutral (BaseTm f)
+| Var_is_neutral : forall {A : ty B} (v : var C A), is_neutral (TmVar v)
+| App_is_neutral : forall {A1 A2 : ty B} (f : tm ar C (A1 ⟶ A2)) (t : tm ar C A1),
+    is_neutral f -> term_isSN t -> is_neutral (f · t).
+
+Lemma beta_red_term_isSN
+      {B : Type}
+      {F : Type}
+      {ar : F -> ty B}
+      {C : con B}
+      {A : ty B}
+      {t1 t2 : tm ar C A}
+      (r : betaRed t1 t2)
+      (Ht1 : term_isSN t1)
+  : term_isSN t2.
+Proof.
+  revert r.
+  revert t2.
+  induction Ht1 as [t1 Ht1 IHt1].
+  intros t2 r.
+  apply acc.
+  intros t' r'.
+  exact (IHt1 t2 r t' r').
+Qed.
+
+Lemma beta_red_neutral
+      {B : Type}
+      {F : Type}
+      {ar : F -> ty B}
+      {C : con B}
+      {A : ty B}
+      {t1 t2 : tm ar C A}
+      (r : betaRed t1 t2)
+      (Ht1 : is_neutral t1)
+  : is_neutral t2.
+Proof.
+  induction r.
+  - apply IHr2.
+    apply IHr1.
+    exact Ht1.
+  - dependent destruction Ht1.
+    constructor.
+    + apply IHr ; assumption.
+    + assumption.
+  - dependent destruction Ht1.
+    constructor.
+    + assumption.
+    + exact (beta_red_term_isSN r H).
+  - inversion Ht1.
+  - dependent destruction Ht1.
+    inversion Ht1.
+Qed.
+
+Lemma wk_neutral
+      {B : Type}
+      {F : Type}
+      {ar : F -> ty B}
+      {C1 C2 : con B}
+      (w : wk C1 C2)
+      {A : ty B}
+      (t : tm ar C2 A)
+      (p : is_neutral t)
+  : is_neutral (wkTm t w).
+Proof.
+  induction t.
+  - constructor.
+  - constructor.
+  - inversion p.
+  - simpl in *.
+    dependent destruction p.
+    constructor.
+    + apply IHt1.
+      assumption.
+    + apply wkTm_isSN.
+      exact H.
+Qed.
+
+Definition map_tm_logical_SN
+           {B : Type}
+           {F : Type}
+           {ar : F -> ty B}
+           {C : con B}
+           {A1 A2 : ty B}
+           (f : tm ar C (A1 ⟶ A2))
+  : tm ar (A1 ,, C) A2
+  := wkTm f (Drop _ (idWk C)) · TmVar Vz.
+
+Definition BetaRed_Wk
+           {B F : Type}
+           {ar : F -> ty B}
+           {C1 C2 : con B}
+           {A : ty B}
+           {t1 t2 : tm ar C2 A}
+           (w : wk C1 C2)
+           (p : betaRed t1 t2)
+  : betaRed (wkTm t1 w) (wkTm t2 w).
+Proof.
+  revert w.
+  revert C1.
+  induction p ; intros C1 w ; simpl.
+  - exact (BetaTrans (IHp1 C1 w) (IHp2 C1 w)).
+  - exact (BetaRew_App_l _ (IHp C1 w)).
+  - exact (BetaRew_App_r _ (IHp C1 w)).
+  - exact (BetaRew_Lam (IHp _ (Keep A1 w))).
+  - simpl.
+    rewrite !wkTm_is_subTm.
+    rewrite subTm_comp.
+    unfold beta_sub.
+    rewrite <- beta_sub_help.
+    rewrite <- subTm_comp.
+    apply BetaBeta.
+Qed.
+
+Lemma Rew_map_tm_logical_SN
+      {B : Type}
+      {F : Type}
+      {ar : F -> ty B}
+      {C : con B}
+      {A1 A2 : ty B}
+      {f1 f2 : tm ar C (A1 ⟶ A2)}
+      (p : betaRed f1 f2)
+  : betaRed (map_tm_logical_SN f1) (map_tm_logical_SN f2).
+Proof.
+  unfold map_tm_logical_SN.
+  apply BetaRew_App_l.
+  apply BetaRed_Wk.
+  exact p.
+Qed.
+
+Lemma neutral_SN
+      {B : Type}
+      {F : Type}
+      {ar : F -> ty B}
+      {C : con B}
+      {A1 A2 : ty B}
+      (f : tm ar C (A1 ⟶ A2))
+      (Hf1 : is_neutral f)
+      (Hf2 : term_isSN f)
+      (t : tm ar C A1)
+      (Ht : term_isSN t)
+  : term_isSN (f · t).
+Proof.
+  revert Hf1 Hf2.
+  revert f.
+  induction Ht as [t Ht IHt].
+  intros f Hf1 Hf2.
+  induction Hf2 as [f Hf2 IHf].
+  apply acc.
+  intros y r.
+  dependent destruction r.
+  - (*assert (f' : tm ar C (A1 ⟶ A)) by admit.
+    assert (t' : tm ar C A1) by admit.
+    assert (p : t3 = f' · t') by admit.
+    assert (H : betaRed t t' + betaRed t t') by admit.
+    subst.
+    destruct H.
+    + apply IHt.
+      apply (IHf f').
+     *)
+    admit.
+  - apply (IHf f2 r).
+    exact (beta_red_neutral r Hf1).
+  - apply (IHt x2 r).
+    + exact Hf1.
+    + apply acc.
+      exact Hf2.
+  - inversion Hf1.
+Admitted.
+
+(** * Properties of the logical relation *)
+
+(** We prove two properties of logical relations, namely that neutral terms satisfy it and that each element that satisfies the relation, is strongly normalizing. We do that by mutual induction. *)
+Lemma neutral_is_logical_SN_and_logical_SN_to_SN
+      {B : Type}
+      {F : Type}
+      {ar : F -> ty B}
+      {A : ty B}
+  : forall {C : con B}
+           (t : tm ar C A),
+    (is_neutral t -> logical_SN t)
+    /\
+    (logical_SN t -> term_isSN t).
+Proof.      
+  induction A as [ b | A1 IHA1 A2 IHA2 ].
+  - simpl.
+    intros C t.
+    split ; intro p.
+    + induction p.
+      * apply baseTm_is_SN.
+      * apply var_is_SN.
+      * apply neutral_SN ; assumption.
+    + assumption.
+  - simpl.
+    intros C t.
+    split ; intro p.
+    + simpl.
+      intros C' w t' q.
+      apply IHA2.
+      constructor.
+      * apply wk_neutral.
+        exact p.
+      * apply IHA1.
+        exact q.
+    + simpl in p.
+      pose (x := wkTm t (Drop A1 (idWk C)) · TmVar Vz).
+      specialize (IHA2 _ x).
+      unfold map_tm_logical_SN in IHA2.
+      assert (logical_SN (wkTm t (Drop A1 (idWk C)) · TmVar Vz)) as w.
+      {
+        apply p.
+        apply IHA1.
+        constructor.
+      }
+      destruct IHA2 as [q IHA2].
+      clear IHA1 q.
+      specialize (IHA2 w).
+      clear p.
+      clear w.
+      dependent induction IHA2.
+      apply acc.
+      intros y Hy.
+      apply (H0 (map_tm_logical_SN y)) ; auto.
+      apply Rew_map_tm_logical_SN.
+      exact Hy.
+Qed.
+
+(** Accessors for these properties *)
+Proposition logical_SN_to_SN
+            {B : Type}
+            {F : Type}
+            {ar : F -> ty B}
+            {A : ty B}
+  : forall {C : con B}
+           {t : tm ar C A}
+           (p : logical_SN t),
+    term_isSN t.
+Proof.
+  intros C t p.
+  apply (neutral_is_logical_SN_and_logical_SN_to_SN t).
+  exact p.
+Qed.
+
+Proposition neutral_is_logical_SN
+            {B : Type}
+            {F : Type}
+            {ar : F -> ty B}
+            {A : ty B}
+  : forall {C : con B}
+           (t : tm ar C A)
+           (p : is_neutral t),
+    logical_SN t.
+Proof.
+  intros C t p.
+  apply (neutral_is_logical_SN_and_logical_SN_to_SN t).
+  exact p.
+Qed.
+
+(** Now we can conclude that variables and base terms satisfy the logical relation *)
+Lemma var_is_logical_SN
+      {B : Type}
+      {F : Type}
+      {ar : F -> ty B}
+      {A : ty B}
+      {C : con B}
+      (v : var C A)
+  : @logical_SN _ _ ar _ _ (TmVar v).
+Proof.
+  apply neutral_is_logical_SN ; cbn.
+  constructor.
+Qed.
+
+Lemma base_is_logical_SN
+      {B : Type}
+      {F : Type}
+      {ar : F -> ty B}
+      {C : con B}
+      (f : F)
+  : @logical_SN _ _ ar C _ (BaseTm f).
+Proof.
+  apply neutral_is_logical_SN ; cbn.
+  constructor.
+Qed.
+
+(** * Closure under beta *)
+
+(** We first define repeat applications. This is basically just a list of terms where they types agree. Note that [repeat_app ar C A1 A2] is a repeated application of a term of type [A1] and it gives a term of type [A2]. *)
+Inductive repeat_app
+          {B : Type}
+          {F : Type}
+          (ar : F -> ty B)
+          (C : con B)
+  : ty B -> ty B -> Type
+  :=
+  | empty : forall (A : ty B), repeat_app ar C A A
+  | add_term : forall (A1 A2 A3 : ty B),
+      tm ar C A2
+      -> repeat_app ar C A1 (A2 ⟶ A3)
+      -> repeat_app ar C A1 A3.
+
+Arguments empty {_ _ _ _ _}.
+Arguments add_term {_ _ _ _ _ _ _} _ _.
+
+(** The semantics of a repeated application *)
+Fixpoint sem
+         {B : Type}
+         {F : Type}
+         {ar : F -> ty B}
+         {C : con B}
+         {A1 A2 : ty B}
+         (ps : repeat_app ar C A1 A2)
+  : tm ar C A1 -> tm ar C A2
+  := match ps with
+     | empty => fun t => t
+     | add_term t qs => fun f => sem qs f · t
+     end.
+
+(** Closure under weakening *)
+Fixpoint wk_repeat_app
+         {B : Type}
+         {F : Type}
+         {ar : F -> ty B}
+         {C1 C2 : con B}
+         {A1 A2 : ty B}
+         (ps : repeat_app ar C2 A1 A2)
+         (w : wk C1 C2)
+  : repeat_app ar C1 A1 A2
+  := match ps with
+     | empty => empty
+     | add_term t qs => add_term (wkTm t w) (wk_repeat_app qs w)
+     end.
+
+Proposition sem_wk_repeat_app
+            {B : Type}
+            {F : Type}
+            {ar : F -> ty B}
+            {C1 C2 : con B}
+            {A1 A2 : ty B}
+            (ps : repeat_app ar C2 A1 A2)
+            (w : wk C1 C2)
+            (t : tm ar C2 A1)
+  : sem (wk_repeat_app ps w) (wkTm t w) = wkTm (sem ps t) w.
+Proof.
+  induction ps as [ | ? ? ? t' qs IHqs ].
+  - reflexivity.
+  - simpl.
+    rewrite IHqs.
+    reflexivity.
+Qed.
+
+(** This lemma expresses that the logical relation is closed under beta reduction *)
+Lemma logical_SN_beta_help
+      {B : Type}
+      {F : Type}
+      {ar : F -> ty B}
+      {C : con B}
+      {A1 A2 A3 : ty B}
+      (f : tm ar (A1 ,, C) A2)
+      (t : tm ar C A1)
+      (Hsub : logical_SN (subTm f (beta_sub t)))
+      (Hf : logical_SN f)
+      (Ht : term_isSN t)
+      (ps : repeat_app ar C A2 A3)
+  : logical_SN (sem ps (λ f · t)).
+Proof.
+  revert ps Ht Hf Hsub.
+  revert t f.
+  revert A1 A2.
+  revert C.
+  induction A3 as [ b | A31 IHA31 A32 IHA32 ] ; intros C A1 A2 t f ps Ht Hf Hsub.
+  - simpl.
+    admit.
+  - intros ? w t' Ht'.
+    specialize (IHA32
+                  _ _ _
+                  (wkTm t w) (wkTm f (Keep A1 w))
+                  (add_term t' (wk_repeat_app ps w))).
+    simpl in IHA32.
+    rewrite <- sem_wk_repeat_app.
+    apply IHA32.
+    + apply wkTm_isSN.
+      exact Ht.
+    + apply wk_logical_SN.
+      exact Hf.
+    + rewrite wkTm_is_subTm.
+      rewrite subTm_comp.
+      simpl ; cbn.
+      rewrite dropSub_is_compSubWk.
+      rewrite <- compSub_compWkSub.
+      simpl ; cbn.
+      rewrite compWkSub_id.
+      rewrite Sub_id_right.
+      unfold beta_sub in Hf.
+      pose (wk_logical_SN w _ Hsub) as l.
+      rewrite wkTm_is_subTm in l.
+      rewrite subTm_comp in l.
+      simpl in l.
+      rewrite Sub_id_left in l.
+      rewrite <- wkTm_is_subTm in l.
+      exact l.
+Admitted.
+
+Lemma logical_SN_beta
+      {B : Type}
+      {F : Type}
+      {ar : F -> ty B}
+      {C : con B}
+      {A1 A2 : ty B}
+      (f : tm ar (A1 ,, C) A2)
+      (t : tm ar C A1)
+      (Hsub : logical_SN (subTm f (beta_sub t)))
+      (Hf : logical_SN f)
+      (Ht : term_isSN t)
+  : logical_SN (λ f · t).
+Proof.
+  exact (logical_SN_beta_help f t Hsub Hf Ht empty).
+Qed.
+
+(** The fundamental theorem of logical relations *)
+Theorem fundamental_thm_relations
+        {B : Type}
+        {F : Type}
+        {ar : F -> ty B}
+        {C1 C2 : con B}
+        (s : sub ar C1 C2)
+        {A : ty B}
+        (t : tm ar C2 A)
+        (p : logical_SN_sub s)
+  : logical_SN (subTm t s).
+Proof.
+  revert p.
+  revert s.
+  revert C1.
+  induction t ; intros C1 s p.
+  - simpl.
+    apply base_is_logical_SN.
+  - simpl.
+    induction s.
+    + inversion v.
+    + dependent induction v ; simpl ; cbn.
+      * simpl in p.
+        exact (Extend_logical_SN_pr2 _ p).
+      * apply IHs.
+        exact (Extend_logical_SN_pr1 _ p).
+  - simpl.
+    intros x w t' Ht'.
+    apply logical_SN_beta.
+    + rewrite wkTm_is_subTm.
+      rewrite !subTm_comp.
+      unfold beta_sub.
+      simpl ; cbn.
+      rewrite !dropSub_is_compSubWk.
+      rewrite <- !compSub_compWkSub.
+      simpl ; cbn.
+      rewrite compWkSub_id.
+      rewrite compWkSub_id.
+      rewrite Sub_id_right.
+      apply IHt.
+      apply Extend_logical_SN ; try assumption.
+      intros ? v.
+      specialize (p _ v).
+      rewrite <- subVar_comp.
+      rewrite <- wkTm_is_subTm.
+      apply wk_logical_SN.
+      assumption.
+    + rewrite wkTm_is_subTm.
+      rewrite subTm_comp.
+      apply IHt.
+      simpl ; cbn ; unfold keepSub.
+      rewrite !dropSub_is_compSubWk.
+      rewrite <- !compSub_compWkSub.
+      simpl ; cbn.
+      rewrite compWkSub_id.
+      apply Extend_logical_SN.
+      * intros ? v.
+        rewrite <- dropSub_is_compSubWk.
+        rewrite <- subVar_comp.
+        pose (wkTm_is_subTm (subVar v s) (Drop A1 w)) as q.
+        simpl in q.
+        rewrite <- q ; clear q.
+        apply wk_logical_SN.
+        apply p.
+      * apply var_is_logical_SN.
+    + apply logical_SN_to_SN.
+      exact Ht'.
+  - specialize (IHt2 _ s p).
+    pose (IHt1 _ s p _ (idWk _) _ IHt2).
+    rewrite wkTm_id in l.
+    exact l.
+Qed.
+
+Lemma logical_SN_wk
+      {B : Type}
+      {F : Type}
+      {ar : F -> ty B}
+      {C1 C2 : con B}
+      (w : wk C1 C2)
+  : @logical_SN_sub _ _ ar _ _ (wkToSub w).
+Proof.
+  intros A v.
+  rewrite <- wkVar_is_subVar.
+  apply neutral_is_logical_SN.
+  constructor.
+Qed.
+
+Lemma idSub_is_logical_SN_sub
+      {B : Type}
+      {F : Type}
+      {ar : F -> ty B}
+      {C : con B}
+  : logical_SN_sub (idSub C ar).
+Proof.
+  rewrite <- wkToSub_id.
+  apply logical_SN_wk.
+Qed.
+
+(** Now we can conclude SN of the STLC *)
+Lemma all_is_logical_SN
+      {B : Type}
+      {F : Type}
+      {ar : F -> ty B}
+      {C : con B}
+      {A : ty B}
+      (t : tm ar C A)
+  : logical_SN t.
+Proof.
+  pose (fundamental_thm_relations (idSub C ar) t) as l.
+  rewrite subTm_id in l.
+  apply l.
+  apply idSub_is_logical_SN_sub.
+Qed.
+
+Theorem BetaRed_SN
+        {B : Type}
+        {F : Type}
+        (ar : F -> ty B)
+        (C : con B)
+        (A : ty B)
+  : Wf (fun (t1 t2 : tm ar C A) => betaRed t1 t2).
+Proof.
+  intro t.
+  apply logical_SN_to_SN.
+  apply all_is_logical_SN.
+Qed.
